Updated; Loaded; Deleted depricatable Updated vList, vDigit and vNatural types; Load compiler tools

tasks/2015.143/MallabaevAzamat/long_number_math/mul.fst
@@ -1,2 +1,0 @@
-val sum: LongNum * LongNum -> LongNum
-let sum a b =
