tasks/task1/2015-143-Mallabaev-Azamat-solution.fst
@@ -1,9 +1,0 @@
-module task1
-  type nat = x:int{x>0}
-  val fibonacci: nat -> Tot nat
-  let rec fibonacci n =
-    if n < 1 then fibonacci (n+2) - fibonacci (n+1)
-    else if n < 3 then 1
-    else fibonacci (n-1) + fibonacci (n-2)
-  
-  let main n = fibonacci n
