compiler/fstar/examples/algorithms/downgrade.fst
@@ -1,0 +1,30 @@
+(*--build-config
+  options:--z3timeout 20;
+  other-files:classical.fst ext.fst set.fsi set.fst heap.fst
+              stperm.fst seq.fsi seq.fst seqproperties.fst arr.fst
+              qs_seq.fst qsort_arr.fst
+--*)
+module Downgrade
+#set-options "--initial_fuel 0 --initial_ifuel 0 --max_fuel 0 --max_ifuel 0"
+open FStar.Array
+open FStar.Seq
+open FStar.SeqProperties
+open FStar.ST
+open FStar.Heap
+type tot_ord (a:Type) = f:(a -> a -> Tot bool){total_order a f}
+
+val qsort_seq : #a:Type -> f:tot_ord a -> x:seq a -> ST (seq a)
+   (fun h -> True)
+   (fun h0 y h1 -> modifies !{} h0 h1 /\ sorted f y /\ permutation a x y)
+let qsort_seq f x =
+  let x_ar = Array.of_seq x in
+  QuickSort.Array.qsort f x_ar;
+  let res = to_seq x_ar in
+  free x_ar;
+  res
+
+val qsort_seq_forget: #a:Type -> f:tot_ord a -> s1:seq a -> Dv (s2:seq a{sorted f s2 /\ permutation a s1 s2})
+let qsort_seq_forget f x =
+  //forget_ST (qsort_seq f) x <-- this doesn't work because of a bug
+  let g = forget_ST (qsort_seq f) in
+  g x
