compiler/fstar/examples/bug-reports/bug022.fst
@@ -1,0 +1,13 @@
+module Bug22
+open Prims.PURE
+
+type exp =
+  | EAbs   : exp -> exp
+  | EFalse : exp
+
+val subst : exp -> Tot exp
+let subst earg =
+  match earg with
+  | EAbs ematch ->
+      EAbs (if 12 = 43 then ematch else EFalse)
+  | _ -> EFalse
