compiler/fstar/examples/bug-reports/bug028.fst
@@ -1,0 +1,10 @@
+
+module Bug28
+open Prims.PURE
+
+val typing : int
+let typing =
+  match 41, 42, Some 43 with
+  | 41, 42, Some 43 -> 0
+  | _, _, _         -> 0
+  end
