compiler/fstar/examples/bug-reports/bug035.fst
@@ -1,0 +1,5 @@
+module Bug35
+open Prims.PURE
+
+assume val factorial : n:nat -> Tot nat
+assume val foo: n:int -> Tot (y:int{y=factorial n})
