compiler/fstar/examples/bug-reports/bug156.fst
@@ -1,0 +1,8 @@
+module Bug156
+
+type tree =
+  | Leaf : tree
+
+val in_tree : int -> tree -> Tot bool
+let in_tree x t = match t with
+  | Leaf n -> false 
