compiler/fstar/examples/bug-reports/bug185.fst
@@ -1,0 +1,39 @@
+module Bug
+
+assume type data
+
+type vk = data
+
+type tag = data
+
+opaque type verified : vk -> data -> Type
+type vkey (p:(data -> Type)) = k:vk{verified k == p}
+
+assume val verify: p:(data -> Type) -> v:vkey p -> d:data -> tag -> Tot (b:bool{b ==> p d})
+
+assume val format : list data -> Tot data
+assume val parse : d:data -> Tot (s : list data {format s = d})
+
+opaque type certified (d:data)
+assume Certified:
+    (forall k. {:pattern (format [k])}
+            certified (format [k]) <==> verified k == certified )
+
+val validate: vkey certified -> list data -> unit
+let rec validate vk0 chain =
+    (match chain with
+    | cert:: chain_tl ->
+        (match parse cert with
+        | [ ctxt; ctag ] ->
+            (match parse ctxt with
+            | [ sender; vk ] -> ()
+            | [ vk ] -> if verify #certified vk0 ctxt ctag then
+              (
+               assert (verified vk == certified);
+               assume (verified vk == certified);
+               validate vk chain_tl
+              )
+                 else ()
+            | _ -> ())
+        | _ -> ())
+    | [] -> ())
