compiler/fstar/examples/bug-reports/bug209.fst
@@ -1,0 +1,31 @@
+module Bug209
+
+(* Need a way to name the implicit t in the body *)
+
+val foo : #t:Type -> x:t -> Lemma (x = x)
+let foo t x = ()
+(* currently getting
+bug209.fst(4,0-59,0) : Error
+Expected a term of type "(t:Type -> x:t -> Lemma (unit))";
+got a function "(fun t x -> ())" (Curried function, but not total)
+ *)
+
+(* There are more ways to write this:
+   Currently type arguments are made implicit by default,
+   whether they are ticket or not *)
+
+val foo2 : t:Type -> x:t -> Lemma (x = x)
+let foo2 t x = ()
+(*
+bug209.fst(17,0-19,3) : Error
+Expected a term of type "(t:Type -> x:t -> Lemma (unit))";
+got a function "(fun t x -> ())" (Curried function, but not total)
+ *)
+
+val foo3 : x:'a -> Lemma (x = x)
+let foo3 t x = ()
+(*
+bug209.fst(28,0-34,0) : Error
+Expected a term of type "('a:Type -> x:'a -> Lemma (unit))";
+got a function "(fun t x -> ())" (Curried function, but not total)
+ *)
