compiler/fstar/examples/extraction/ghostTest.fst
@@ -1,0 +1,44 @@
+(*--build-config
+ other-files: ext.fst set.fsi set.fst heap.fst st.fst all.fst ghost.fst list.fst
+  --*)
+
+
+module GhostTest
+
+open Ghost
+open List
+type sizedListNonGhost =
+| MkSListNG: maxsize:nat->  cont:(list int){length cont < (maxsize)} -> sizedListNonGhost
+
+val aSizedListNG :  sizedListNonGhost
+let aSizedListNG = MkSListNG ( 2) [1]
+
+type sizedList =
+| MkSList: maxsize:(erased nat)->  cont:(list int){length cont < (reveal maxsize)} -> sizedList
+
+val aSizedList : sizedList
+let aSizedList =  MkSList (hide 2) [1]
+
+assume val effectfulIncr : nat -> St nat
+
+val someNat : nat -> nat
+let someNat n =
+  let _ = (hide (effectfulIncr n)) in n
+
+assume val pureIncr : nat -> Tot nat
+
+val someNat2 : nat -> nat
+let someNat2 n =
+  let _ = (hide (pureIncr n)) in n
+
+open Heap
+type llist : Type -> Type
+type rep : #a:Type -> heap -> llist a  -> list a -> Type
+
+
+val llrev : #a:Type -> l:(llist a) -> el:erased (list a)
+    -> ST ((llist a)*(erased (list a)))
+        (fun m -> rep m l (reveal el))
+        (fun _ rl m1 -> rep m1 (fst rl) (reveal (snd rl)))
+
+let llev l el = admit ()
