compiler/fstar/examples/low-level/MD5.fst
@@ -1,0 +1,176 @@
+(*--build-config
+    other-files:ext.fst set.fsi set.fst heap.fst st.fst all.fst list.fst  stack.fst listset.fst
+    ghost.fst located.fst lref.fst stackAndHeap.fst sst.fst rstWhile.fst constr.fst word.fst seq.fsi seq.fst array.fsi
+     array.fst MD5Common.fst arrayAlgos.fst
+  --*)
+
+(*Why is MD5 so? Why did its designer(s) think
+  it was a good way to convolute bits?
+  Is there a principle behind its design? or just random convolutery?
+  *)
+module MD5
+open RSTWhile
+open RST
+open MVector
+open Set
+open MachineWord
+open MD5Common
+open StackAndHeap
+open Lref  open Located
+open Seq
+open RSTArray
+open ArrayAlgos
+open Ghost
+
+
+assume val cloneAndPad :
+  r:(sstarray word)
+  -> rcloned :(sstarray word)
+  -> Mem unit
+      (fun m -> (liveArr m r) /\ (liveArr m rcloned))
+      (fun m0 rp m1  -> (liveArr m0 r) /\ (liveArr m1 rcloned)
+          /\ (liveArr m1 r)
+          /\ (glength rcloned m1) = psize ((glength r m0))
+          /\ prefixEqual
+                (lookupRef (reveal (asRef r)) m0)
+                (lookupRef (reveal (asRef rcloned)) m1)
+                ((glength r m0)))
+        (hide empty)
+
+val processChunk :
+ ch:(sstarray word)
+ -> offset:nat
+ -> acc:(sstarray word)
+ -> WNSC unit
+    (requires (fun m -> (liveArr m ch)
+              /\ (liveArr m acc) /\ ch =!= acc
+              /\ offset + 16 <= ((glength ch m))
+              /\ 4 = ((glength acc m))
+              ))
+    (ensures (fun m0 _ m1 -> (liveArr m1 ch)
+              /\ (liveArr m1 acc) /\ ch =!= acc
+              /\ 4 = ((glength acc m1))
+              (*/\ lookupRef  ch m0 = lookupRef ch m1*)
+              ))
+    (eonly acc)
+
+
+let processChunk ch offset acc =
+  let li = ralloc #nat 0 in
+  scopedWhile1
+    li
+    (fun liv -> liv < 64)
+    (fun m -> True
+              /\ (liveArr m ch)
+              /\ (liveArr m acc)
+              /\ offset + 16 <= ((glength ch m))
+              /\ 4 = ((glength acc m))
+              /\ refIsLive li m /\ lookupRef li m < 65
+              )
+    (eunion (only li) (eonly acc))
+    (*allRefs ; why does this not work?*)
+    (fun u ->
+      let liv = memread li in
+      let vA = readIndex acc iA in
+      let vB = readIndex acc iB in
+      let vC = readIndex acc iC in
+      let vD = readIndex acc iD in
+      let fF:word = funFGHI liv vB vC vD in
+      let g:(n:nat{n<16}) = idx liv liv in
+      writeIndex acc iD vC;
+      writeIndex acc iA vD;
+      let mg = readIndex ch (offset+g) in
+      let vBr = wmodAdd vA  (wmodAdd fF ( wmodAdd(consts liv)  mg)) in
+      writeIndex acc iB (wmodAdd vB (leftrotate (rots liv) vBr));
+      memwrite li (liv+1))
+
+val mainLoop :
+ ch:(sstarray word)
+ -> un:unit
+ -> WNSC (s:(seq word){Seq.length s = 4})
+    (requires (fun m -> (liveArr m ch)
+          /\ divides 16 ((glength ch m))))
+    (ensures (fun m0 _ m1 -> True /\ (liveArr m1 ch)))
+    (hide empty)
+
+let mainLoop ch u =
+  let offset = ralloc #nat 0 in
+  let acc =  screateSeq initAcc in
+  let chl = RSTArray.length ch in
+  scopedWhile1
+    offset
+    (fun offsetv-> offsetv +16 <= chl)
+    (fun m -> True
+              /\ (liveArr m ch)
+              /\ (liveArr m acc)
+              /\ refIsLive offset m
+              /\ (glength ch m) = chl
+              /\ 4 = ((glength acc m))
+              )
+    (eunion (only  offset) (eonly acc))
+    (fun u ->
+        let offsetv = memread offset in
+        processChunk ch offsetv acc;
+        memwrite offset (offsetv + 16));
+  (to_seq acc)
+
+val allZeros : n:nat -> Tot (s:(seq word){Seq.length s = n})
+let allZeros n = Seq.create n w0
+
+val mD5 :
+ ch:(sstarray word)
+ -> WNSC (s:(seq word){Seq.length s = 4})
+    (fun m -> True /\ (liveArr m ch))
+    (fun m0 _ m1 -> True /\ (liveArr m1 ch))
+    (hide empty)
+
+let mD5 ch =
+  let chl = RSTArray.length ch in
+  let z:nat =0 in
+  let clonedCh = screate  (psize chl) w0 in
+  cloneAndPad ch clonedCh;
+  withNewScope
+    #_
+    #(fun m -> (liveArr m ch) /\ (liveArr m clonedCh)
+        /\ divides 16 ((glength clonedCh m)) )
+    #(fun m0 _ m1 -> True /\ liveArr m1 ch)
+    #(hide empty)
+    (mainLoop clonedCh)
+
+(*open Example2
+
+val mD53 : n:nat
+ -> ch:(sstarray word)
+ -> WNSC (vector word 4)
+    (fun m -> True /\ refIsLive (asRef ch) m)
+    (fun m0 _ m1 -> True /\ refIsLive (asRef ch) m1)
+    (empty)
+
+let mD53 n ch =
+  let clonedCh = screateArray (allZeros (psize n)) in
+  cloneAndPad ch clonedCh;
+  withNewScope4
+    (mainLoop clonedCh)*)
+
+
+val mD52 : n:nat
+ -> ch:(sstarray word)
+ -> WNSC  (s:(seq word){Seq.length s = 4})
+    (fun m -> True /\ (liveArr m ch))
+    (fun m0 _ m1 -> True /\ (liveArr m1 ch))
+    (hide empty)
+
+let mD52 n ch =
+  let clonedCh = screate (psize n) w0 in
+  cloneAndPad ch clonedCh;
+    pushRegion ();
+      let mdd5 = mainLoop clonedCh () in
+    popRegion (); mdd5
+
+
+(*can we run this program and compare it agains standard implementations?
+  That at least needs the following:
+  1) implementations of admitted functions, e.g. padding
+  2) implementations of =
+  3) (optionally, for efficiency) proper "Extraction" of word to native words in OCaml
+*)
