compiler/fstar/examples/stateful_bignum/bigint_st.fst
@@ -1,0 +1,324 @@
+module Bigint
+
+open IntLib
+open Limb
+open FStar.Seq
+open FStar.SeqProperties
+open FStar.All
+open FStar.ST
+open FStar.Heap
+open FStar.Array
+
+(* TODO : stabilize the type definitions *)
+(* Int types *)
+type int64 = int
+type integer = int
+type u8 = int
+
+let ocaml63 = 63
+
+(* Maps the index of the integer data to the theoretic bit size of the cell *)
+type template = nat -> Tot (n:pos{ n < ocaml63 })
+type template_const = t:template{ forall (n:nat). t n = t 0 }
+
+(* Sized integer *)
+type tint (max:nat) = (size:nat{ size < max } & content:int{ Bitsize content size })
+
+(* Sized ST array *)
+type tarray (max:nat) = array (tint max)
+
+(* Big integer type *)
+type bigint = 
+  | Bigint63 : data:tarray ocaml63 -> t:template -> bigint
+
+val wordSize: bigint -> Tot pos
+let wordSize b = 
+  match b with
+    | Bigint63 _ _ -> ocaml63
+
+type SameFormat (ha:heap) (hb:heap) (a:bigint) (b:bigint) = 
+  (contains ha (Bigint63.data a) /\ contains hb (Bigint63.data b))
+  /\ (Bigint63.t a = Bigint63.t b) 
+  /\ (Seq.length (sel ha (Bigint63.data a)) = Seq.length (sel hb (Bigint63.data b)))
+
+type inHeap (h:heap) (b:bigint) = b2t (contains h (Bigint63.data b))
+
+(* Getters *)
+
+(* Logical only *)
+assume logic val getLength : 
+	       h:heap -> b:bigint{ inHeap h b } -> 
+	       Tot (len:nat{ len = Seq.length (sel h (Bigint63.data b)) })
+
+assume logic val getSize : 
+	       h:heap -> b:bigint{ inHeap h b } -> i:nat{ i < getLength h b } -> 
+	       Tot (s:nat{s = dfst (Seq.index (sel h (Bigint63.data b)) i) /\  s < (wordSize b)})
+
+assume logic val getValue :
+	       h:heap -> b:bigint{ inHeap h b } -> i:nat{ i < getLength h b } ->
+	       Tot (v:int{ v = dsnd (Seq.index (sel h (Bigint63.data b)) i)})
+
+assume logic val getContent :
+	       h:heap -> b:bigint{ inHeap h b } -> i:nat{ i < getLength h b } ->
+	       Tot (v:tint (wordSize b){ v = (Seq.index (sel h (Bigint63.data b)) i)})
+
+val size_of_value_lemma:
+  h:heap -> b:bigint{ inHeap h b } -> i:nat{ i < getLength h b } -> 
+  Lemma
+    (requires (True))
+    (ensures (Bitsize (getValue h b i) (getSize h b i)))
+let size_of_value_lemma h b i = 
+  erase (
+      let v = getContent h b i in
+      assert ( v = (Seq.index (sel h (Bigint63.data b)) i) /\ True);
+      assert ( dfst v = dfst (Seq.index (sel h (Bigint63.data b)) i) /\ True);
+      ()
+    )
+
+(* Concrete getters *)
+val get_content: 
+  b:bigint -> i:nat ->
+  ST (tint (wordSize b))
+     (requires (fun h -> (inHeap h b)
+			 /\ (i < getLength h b)))
+     (ensures (fun h0 v h1 -> (inHeap h1 b)
+			      /\ (h1==h0)
+			      /\ (i < getLength h1 b)
+			      /\ (v = getContent h1 b i)))
+let get_content b i =
+  match b with 
+  | Bigint63 data t ->
+     Array.index data i
+
+val get_length:
+  b:bigint ->
+  ST nat
+     (requires (fun h -> (inHeap h b)))
+     (ensures (fun h0 l h1 -> (h0 == h1) 
+			      /\ (inHeap h0 b)
+			      /\ (l = getLength h0 b)))
+let get_length b =
+  match b with
+  | Bigint63 data t -> Array.length data		 
+
+val get: 
+  b:bigint -> n:nat -> 
+  ST int
+     (requires (fun h -> inHeap h b /\ n < getLength h b))
+     (ensures (fun h0 v h1 -> (h0==h1)
+			      /\ (inHeap h1 b)
+			      /\ (n < getLength h1 b)
+			      /\ (v = getValue h1 b n /\ Bitsize v (getSize h1 b n))
+      ))
+let get b n =
+  match b with
+  | Bigint63 data t ->
+     let (|size,v|) = (Array.index data n) in v
+
+val getTemplate: bigint -> Tot template
+let getTemplate b =
+  match b with
+  | Bigint63 _ t -> t
+
+(* Setter *)
+val updateBigint:
+  b:bigint -> idx:nat -> v:tint ocaml63 -> 
+  ST unit
+     (requires (fun h -> (contains h (Bigint63.data b))
+			 /\ (idx < Seq.length (sel h (Bigint63.data b)))))
+     (ensures (fun h0 u h1 -> 
+	       (idx < Seq.length (sel h0 (Bigint63.data b)))
+               /\ (contains h1 (Bigint63.data b))
+	       /\ (h1==Heap.upd h0 (Bigint63.data b) (Seq.upd (sel h0 (Bigint63.data b)) idx v))
+		 
+      ))
+let updateBigint b idx v =
+  match b with
+  | Bigint63 data _ ->
+     Array.upd data idx v
+
+val update_bigint_lemma:
+  h0:heap -> h1:heap -> b:bigint{ inHeap h1 b /\ inHeap h0 b }  -> idx:nat{ idx < getLength h0 b } -> v:tint ocaml63 -> 
+  Lemma
+    (requires (h1 == Heap.upd h0 (Bigint63.data b) (Seq.upd (sel h0 (Bigint63.data b)) idx v)))
+    (ensures ( (getLength h1 b = getLength h0 b)
+	       /\ (getValue h1 b idx = dsnd v) 
+	       /\ (getSize h1 b idx = dfst v)
+	       /\ (forall (i:nat). (i < getLength h1 b /\ i <> idx) ==> 
+		     (getValue h1 b i = getValue h0 b i /\ getSize h1 b i = getSize h0 b i) )
+	       /\ (modifies !{Bigint63.data b} h0 h1) ))
+let update_bigint_lemma h0 h1 b idx v = ()
+
+type EqualBigint (a:bigint) (b:bigint) (ha:heap) (hb:heap) =
+  (contains ha (Bigint63.data a)) 
+  /\ (contains hb (Bigint63.data b))
+  /\ (getLength ha a = getLength hb b)
+  /\ (forall (i:nat). i < getLength ha a ==> getValue ha a i = getValue hb b i)
+  /\ (forall (i:nat). i < getLength ha a ==> getSize ha a i = getSize hb b i)
+  /\ (Bigint63.t a = getTemplate b)
+
+opaque val copy:
+  a:bigint ->
+  ST bigint
+     (requires (fun h -> inHeap h a /\ getLength h a > 0))
+     (ensures (fun h0 b h1 ->
+       (inHeap h0 a)
+       /\ (inHeap h1 b)
+       /\ not(contains h0 (Bigint63.data b))
+       /\ (EqualBigint a b h0 h1)
+       /\ (modifies !{} h0 h1)
+     ))
+let copy a =
+  Bigint63 (Array.copy (Bigint63.data a)) (Bigint63.t a)
+
+(* Normalized big integer type *)
+type Normalized (h:heap) (b:bigint{ inHeap h b })  =
+  (forall (n:nat). n < getLength h b ==> getSize h b n <= (Bigint63.t b) n)
+
+type IsNull (h:heap) (b:bigint{ inHeap h b }) =
+  (forall (n:nat). n < getLength h b ==> getValue h b n = 0)
+
+(* Zeros and ones *)
+val zero_tint: z:tint ocaml63{ dsnd z = 0 }
+let zero_tint = (|0, 0|)
+
+val one_tint: z:tint ocaml63{ dsnd z = 1 }
+let one_tint = (|1, 1|)
+
+let mk_zero_bigint size template =
+  Bigint63 (Array.create size zero_tint) template
+
+let mk_one_bigint size template =
+  let one = Bigint63 (Array.create size zero_tint) template in
+  updateBigint one 0 one_tint;
+  one
+
+val mk_tint: a:bigint -> size:nat{ size < wordSize a } -> value:int{ Bitsize value size } -> 
+	     Tot (z:tint (wordSize a))
+let mk_tint a size value =
+  match a with
+  | Bigint63 _ _ -> 
+     (|size, value|)
+
+opaque val extend :
+  a:bigint -> len:pos ->
+  ST bigint
+    (requires (fun h ->
+      (inHeap h a)
+      /\ (len >= getLength h a)
+     ))
+    (ensures (fun h0 b h1 ->
+      (inHeap h0 a)
+      /\ (inHeap h1 b)
+      /\ (Bigint63.data b <> Bigint63.data a)
+      /\ (modifies !{} h0 h1)
+      /\ (len >= getLength h0 a)
+      /\ (getLength h1 b = len)
+      /\ (Seq.Eq (sel h0 (Bigint63.data a)) (Seq.slice (sel h1 (Bigint63.data b)) 0 (getLength h0 a)))
+      /\ (forall (i:nat). (i >= getLength h0 a /\ i < len)
+	  ==> Seq.index (sel h1 (Bigint63.data b)) i = zero_tint)
+     ))
+let extend a len =
+  let len_a = get_length a in
+  let b = Bigint.mk_zero_bigint len (Bigint63.t a) in
+  Array.blit (Bigint63.data a) 0 (Bigint63.data b) 0 len_a;
+  b
+
+#reset-options
+
+val populate_tarray : 
+  t:array int -> templ:template -> max:nat -> len:nat -> a:tarray max ->
+  ST unit
+    (requires (fun h -> True))
+    (ensures (fun h0 _ h1 -> True))
+let rec populate_tarray t templ max len a = 
+  match len with
+  | 0 -> ()
+  | _ -> 
+     let i = len - 1 in
+     Array.upd a i (|templ i, Array.index t i|);
+     populate_tarray t templ max (len-1) a
+
+val mk_tarray : 
+  t:array int -> templ:template -> max:nat ->
+  ST (tarray max)
+    (requires (fun h -> True))
+    (ensures (fun h0 s h1 -> True))
+let mk_tarray t tmpl max =
+  let len = Array.length t in
+  let a = Array.create len zero_tint in
+  populate_tarray t tmpl max 0 a;
+  a
+
+val populate_array : 
+  max:pos -> t:tarray max -> len:nat -> a:array int ->
+  ST unit
+    (requires (fun h -> True))
+    (ensures (fun h0 _ h1 -> True))
+let rec populate_array max t len a =
+  match len with
+  | 0 -> ()
+  | _ -> 
+     let i = len - 1 in
+     let ti = Array.index t i in
+     Array.upd a i (dsnd ti);
+     populate_array max t (len-1) a
+
+val mk_array : 
+  max:pos -> t:tarray max ->
+  ST (array int)
+    (requires (fun h -> True))
+    (ensures (fun h0 s h1 -> True))
+let mk_array max t =
+  let len = Array.length t in
+  let a = Array.create len 0 in
+  populate_array ocaml63 t 0 a;
+  a
+
+(*
+(* Pool of free arrays for temporary computation *)
+type array_pool = { free_arrays: ref (list (tarray ocaml63));
+	      array_size: ref pos;
+	      pool_size: ref nat }
+
+val pool: array_pool
+let pool = { free_arrays = ref [];
+	     array_size = ref 1;
+	     pool_size = ref 0; }
+
+//val initialize_pool: max:nat -> array_size:pos -> ST unit
+let initialize_pool max size =
+  match max with
+  | 0 ->
+     pool.array_size := size;
+     pool.pool_size := max
+  | _ ->
+     pool.free_arrays := (Array.create size zero_tint)::!(pool.free_arrays)
+
+val get_from_pool : size:nat -> ST (tarray ocaml63)
+				   (requires (fun h -> True))
+				   (ensures (fun h0 t h1 -> 
+					     (True)))
+let get_from_pool size =
+  match !(pool.free_arrays), size with
+  | hd::tl, _ -> 
+     if size = !pool.array_size then
+       (pool.free_arrays := tl;
+	hd)
+     else 
+       (
+	 (* Issue warning *)
+	 (* Create pool mapping size to fresh array of that size ? *)
+	 Array.create size zero_tint
+       )
+  | _, _ -> 
+     (* Issue warning *)
+     (* Increase pool size *)
+     Array.create size zero_tint		 
+
+val return_to_pool : tarray ocaml63 -> ST unit
+				     (requires (fun h -> True ))
+				     (ensures (fun h0 u h1 -> True))
+let return_to_pool a =
+  pool.free_arrays := a::!(pool.free_arrays)
+*)
