compiler/fstar/lib/char.fst
@@ -1,0 +1,5 @@
+module FStar.Char
+
+assume val lowercase: char -> char
+assume val uppercase: char -> char
+assume val int_of_char: char -> int
