tasks/2015.143/MallabaevAzamat/VDigit.fst
@@ -1,0 +1,18 @@
+module VDigit
+
+open VList
+
+val isDigit: int * int -> Tot bool
+let isDigit (v, s) = v < s && 0 < v
+
+type vDigit = t:(int * int) {isDigit t}
+
+val sum: vDigit -> vDigit -> Tot vDigit
+let sum = function
+  | (v1, s1) -> function
+  | (v2, s2) -> ((v1 + v2), (s1 + s2))
+
+val reduce: (int -> int) -> vDigit -> x:Tot (vList vDigit) {x <> VEmpty}
+let reduce rule = 
+  VCons (v, rule level) VEmpty
+
