tasks/2015.143/MallabaevAzamat/VList.fst
@@ -1,0 +1,46 @@
+﻿module VList
+
+type vList 'a =
+   | VEmpty : vList 'a
+   | VCons  : 'a -> vList 'a -> vList 'a
+
+val length: vList 'a -> Tot int
+let rec length = function
+  | VEmpty    -> 0
+  | VCons _ t -> 1 + length t
+
+val isEmpty: vList 'a -> Tot bool
+let isEmpty = function
+  | VEmpty -> true
+  | _      -> false
+
+val isCons: vList 'a -> Tot bool
+let isCons = function
+  | VCons _ _ -> true
+  | _         -> false
+
+val head: l:vList 'a {isCons l} -> Tot 'a
+let head = function
+  | VCons h _ -> h
+
+val tail: l:vList 'a {isCons l} -> Tot (vList 'a)
+let tail = function
+  | VCons _ t -> t
+
+val fold: 'b -> ('a -> 'b -> 'b) -> vList 'a -> Tot 'b
+let rec fold st f = function
+  | VEmpty    -> st
+  | VCons h t -> fold (f h) f t
+
+val map: ('a -> Tot 'b) -> vList 'a -> Tot (vList 'b)
+let rec map f = function
+  | VEmpty    -> VEmpty
+  | VCons h t -> VCons (f h) (map f t)
+
+val rev: vList 'a -> Tot (vList 'a)
+let rev f = fold VEmpty VCons f
+
+val append: vList 'a -> vList 'a -> Tot (vList 'a)
+let rec append = function
+  | VEmpty    -> fun l -> l
+  | VCons h t -> fun l -> VCons h (append t l)
