tasks/2015.143/MallabaevAzamat/VNatural.fst
@@ -1,0 +1,17 @@
+﻿module VNatural
+
+open VList
+open VDigit
+
+type vNatural = x:(vList vDigit){x <> VEmpty /\ x <> VCons 0 _}
+
+val sum: vNatural -> vNatural -> Tot vNatural
+let sum a b =
+  let rA = rev a
+  let rB = rev b
+  let rSum = function
+    | VEmpty -> fun b -> b
+    | VCons h t -> function
+      | Vempty      -> VCons h t
+      | VCons hh tt -> (VDigit.sum h hh) (rSum t tt)
+  rev (rSum rA rB)
