tasks/2015.143/MallabaevAzamat/long_number_math/digit.fst
@@ -1,1 +1,0 @@
-type Digit = d:int {d >= 0 \/ d < 10}
