tasks/2015.143/MallabaevAzamat/long_number_math/list.fst
@@ -1,3 +1,0 @@
-type List<'a> =
-| Nil
-| Cons of 'a
