tasks/2015.143/MallabaevAzamat/long_number_math/long_num.fst
@@ -1,1 +1,0 @@
-type LongNum = x: Sign * y: List<Digit> { (y = Nil /\ x = Plus) \/ (y = Cons(a, _) /\ a <> 0) }
